map/MapA.v
@@ -112,28 +112,28 @@ Module MapAS. Section MapAS.
   Section spec.
     Context (u : univ_id).
     Definition init_spec : fspec :=
-      w_fspec u
+      wsim_fspec u
         (fspec_simple
           (λ sz : nat,
             (λ varg, ⌜varg = [Vint sz]↑ ∧ (8 * (Z.of_nat sz) < modulus_64)%Z⌝ ∗ pending,
               λ vret, ⌜vret = Vundef↑⌝ ∗ initial_points_tos sz)))%I.
 
     Definition get_spec: fspec :=
-      w_fspec u
+      wsim_fspec u
         (fspec_simple
           (λ '(k, v),
             (λ varg, ⌜varg = [Vint k]↑⌝ ∗ points_to k v,
               λ vret, ⌜vret = (Vint v)↑⌝ ∗ points_to k v)))%I.
 
     Definition set_spec: fspec :=
-      w_fspec u
+      wsim_fspec u
         (fspec_simple
           (λ '(k, w, v),
             (λ varg, ⌜varg = [Vint k; Vint v]↑⌝ ∗ points_to k w,
               λ vret, ⌜vret = Vundef↑⌝ ∗ points_to k v)))%I.
 
     Definition set_by_user_spec: fspec :=
-      w_fspec u
+      wsim_fspec u
         (fspec_simple
           (λ '(k, w),
             (λ varg, ⌜varg = [Vint k]↑⌝ ∗ points_to k w,
@@ -210,5 +210,5 @@ Module MapA. Section MapA.
   Definition init_cond : iProp Σ :=
     (MapAS.initial_map ∗ MapMS.pending)%I.
 
-  Definition t sp := Seal.sealing CRIS (SMod.to_hmod emp sp Mod).
+  Definition t sp := Seal.sealing CRIS (SMod.to_hmod sp Mod).
 End MapA. End MapA.
